copyright and geometric

Library/Model/Geometric.dfy
@@ -1,38 +1,55 @@
+/*******************************************************************************
+*  Copyright by the contributors to the Dafny Project
+*  SPDX-License-Identifier: MIT
+*******************************************************************************/
+
 include "Monad.dfy"
 include "RandomNumberGenerator.dfy"
+include "WhileAndUntil.dfy"
+include "Independence.dfy"
 
 module Geometric {
   import opened Monad
   import opened RandomNumberGenerator
+  import opened WhileAndUntil
+  import opened Independence
 
   /************
    Definitions  
   ************/
 
   // Equation (4.17)
-  function ProbGeometricIter(b: bool, n: nat): Hurd<(bool, nat)> {
-    var f := (b': bool) => Return(b', n + 1);
-    Bind(Deconstruct, f)
+  function ProbGeometricIter(): ((bool, int)) -> Hurd<(bool, int)> {
+    var g := (t: (bool, int)) => 
+      var f := (b': bool) => Return((b', t.1 + 1));
+      Bind(Deconstruct, f);
+    g
   }  
 
   // Equation (4.18)
-  function ProbGeometric(): Hurd<nat> {
-    var fst := ((x, _): (bool, nat)) => x;
-    var f := ((b, n): (bool, nat)) => Return(n - 1);
-    Bind(ProbWhile(fst, ProbGeometricIter(true, 0)), f)
+  function ProbGeometric(): Hurd<int> {
+    var fst := (t: (bool, int)) => t.0;
+    var f := (t: (bool, int)) => Return(t.1 - 1);
+    ProbWhileGeometricTerminates();
+    var g := ProbWhile(fst, ProbGeometricIter(), (true, 0));
+    Bind(g, f)
   }
 
   /*******
    Lemmas  
   *******/
 
+  lemma {:axiom} ProbWhileGeometricTerminates()
+    ensures 
+      var fst := (t: (bool, int)) => t.0;
+      ProbWhileTerminates(ProbGeometricIter(), fst)
+
   // Equation (4.19)
   lemma {:axiom} ProbGeometricIsIndepFn()
-    ensures IsIndepFn(ProbGeometric)
+    ensures IsIndepFn(ProbGeometric())
   
   // Equation (4.20)
   lemma {:axiom} ProbGeometricCorrectness()
-    ensures 
 
 }
 
